src/HeapState.v
@@ -7,9 +7,9 @@ Require Import
   Coq.FSets.FMapFacts
   Coq.Structures.DecidableTypeEx.
 
-Module HeapState (M : WSfun N_as_DT).
+Module HeapState (M : WSfun Ptr_as_DT).
 
-Module Import FMapExt := FMapExt N_as_DT M.
+Module Import FMapExt := FMapExt Ptr_as_DT M.
 Module P := FMapExt.P.
 Module F := P.F.
 
@@ -44,35 +44,40 @@ Definition newHeapState :=
   {| resvs := M.empty _
    ; bytes := M.empty _ |}.
 
-Definition within (addr : N) (len : N) (a : N) : Prop :=
-  addr <= a < addr + len.
+Definition within `(addr : Ptr A) (len : N) (a : Ptr A) : Prop :=
+  addr <= a < plusPtr addr len.
 Hint Unfold within.
 
-Definition within_bool (addr : N) (len : N) (a : N) : bool :=
-  ((addr <=? a) && (a <? addr + len))%bool.
+Definition within_bool `(addr : Ptr A) (len : N) (a : Ptr A) : bool :=
+  ((addr <=? a) && (a <? plusPtr addr len))%bool.
 Hint Unfold within_bool.
 
-Definition fits (addr1 len1 addr2 len2 : N) : Prop :=
-  within addr1 len1 addr2 /\ addr2 + len2 <= addr1 + len1.
+Corollary within_zero : forall A (n m : Ptr A),
+  within_bool n 0 m = false.
+Proof. intros; destruct (Nlt_dec m n); nomega. Qed.
+
+Definition fits `(addr1 : Ptr A) (len1 : N) (addr2 : Ptr A) (len2 : N) : Prop :=
+  within addr1 len1 addr2 /\ plusPtr addr2 len2 <= plusPtr addr1 len1.
 Hint Unfold fits.
 
-Definition fits_bool (addr1 len1 addr2 len2 : N) : bool :=
-  (within_bool addr1 len1 addr2 && (addr2 + len2 <=? addr1 + len1))%bool.
+Definition fits_bool `(addr1 : Ptr A) (len1 : N) (addr2 : Ptr A) (len2 : N) : bool :=
+  (within_bool addr1 len1 addr2 &&
+   (plusPtr addr2 len2 <=? plusPtr addr1 len1))%bool.
 Hint Unfold fits_bool.
 
-Definition overlaps (addr len addr2 len2 : N) : Prop :=
-  addr < addr2 + len2 /\ addr2 < addr + len.
+Definition overlaps `(addr : Ptr A) (len : N) (addr2 : Ptr A) (len2 : N) : Prop :=
+  addr < plusPtr addr2 len2 /\ addr2 < plusPtr addr len.
 Hint Unfold overlaps.
 
-Definition overlaps_bool (addr len addr2 len2 : N) : bool :=
-  ((addr <? addr2 + len2) && (addr2 <? addr + len))%bool.
+Definition overlaps_bool `(addr : Ptr A) (len : N) (addr2 : Ptr A) (len2 : N) : bool :=
+  ((addr <? plusPtr addr2 len2) && (addr2 <? plusPtr addr len))%bool.
 Hint Unfold overlaps_bool.
 
-Lemma not_overlaps_sym : forall addr1 len1 addr2 len2,
+Lemma not_overlaps_sym : forall A (addr1 addr2 : Ptr A) len1 len2,
   ~ overlaps addr1 len1 addr2 len2 <-> ~ overlaps addr2 len2 addr1 len1.
 Proof. autounfold; nomega. Qed.
 
-Corollary not_overlaps_trans : forall a b x y z,
+Corollary not_overlaps_trans : forall A (a x : Ptr A) b y z,
   z < y -> ~ overlaps a b x y -> ~ overlaps a b x z.
 Proof.
   unfold not; intros.
@@ -81,26 +86,26 @@ Proof.
 Qed.
 
 Definition find_free_block (len : Size) `(r : M.t (Ptr A)) : Comp (Ptr A) :=
-  { addr : N | P.for_all (fun a sz => negb (overlaps_bool a sz addr len)) r }.
+  { addr : Ptr A | P.for_all (fun a sz => negb (overlaps_bool a sz addr len)) r }.
 
-Definition keep_range {elt} (addr : M.key) (len : N) : M.t elt -> M.t elt :=
+Definition keep_range {elt} `(addr : Ptr A) (len : N) : M.t elt -> M.t elt :=
   keep_keys (within_bool addr len).
 
-Definition drop_range {elt} (addr : M.key) (len : N) : M.t elt -> M.t elt :=
+Definition drop_range {elt} `(addr : Ptr A) (len : N) : M.t elt -> M.t elt :=
   keep_keys (fun p => negb (within_bool addr len p)).
 
-Definition copy_bytes {elt} (from to : M.key) (len : N)
+Definition copy_bytes {elt A} (from to : Ptr A) (len : N)
            (mfrom mto : M.t elt) : M.t elt :=
   P.update (drop_range to len mto)
            (M.fold (fun k e rest =>
                       If within_bool from len k
-                      Then M.add (k - from + to) e rest
+                      Then M.add (plusPtr to (k - from)) e rest
                       Else rest)
                    mfrom (M.empty _)).
 
-Program Instance copy_bytes_Proper :
+Program Instance copy_bytes_Proper : forall A,
   Proper (eq ==> eq ==> eq ==> M.Equal ==> M.Equal ==> @M.Equal elt)
-         copy_bytes.
+         (copy_bytes (A:=A)).
 Obligation 1.
   relational.
   unfold copy_bytes, drop_range, keep_range, keep_keys.
@@ -116,15 +121,16 @@ Obligation 1.
     rewrite add_associative.
       reflexivity.
     intros.
-    apply N.add_cancel_r in H0.
+    unfold plusPtr in H0.
     nomega.
 Qed.
 
-Lemma copy_bytes_mapsto : forall elt k (e : elt) addr1 addr2 len m1 m2,
-  M.MapsTo k e (copy_bytes addr1 addr2 len m1 m2)
-    <-> (If within_bool addr2 len k
-         Then M.MapsTo (k - addr2 + addr1) e m1
-         Else M.MapsTo (elt:=elt) k e m2).
+Lemma copy_bytes_mapsto :
+  forall elt k (e : elt) A (addr1 addr2 : Ptr A) len m1 m2,
+    M.MapsTo k e (copy_bytes addr1 addr2 len m1 m2)
+      <-> If within_bool addr2 len k
+          Then M.MapsTo (plusPtr addr1 (k - addr2)) e m1
+          Else M.MapsTo (elt:=elt) k e m2.
 Proof.
   unfold copy_bytes, drop_range, keep_range, keep_keys,
          const, not, compose.
@@ -189,11 +195,12 @@ Proof.
   contradiction.
 Qed.
 
-Lemma copy_bytes_find : forall a1 a2 k l elt (m1 m2 : M.t elt),
-  M.find k (copy_bytes a1 a2 l m1 m2)
-    = If within_bool a2 l k
-      Then M.find (k - a2 + a1) m1
-      Else M.find k m2.
+Lemma copy_bytes_find :
+  forall A (a1 a2 : Ptr A) k l elt (m1 m2 : M.t elt),
+    M.find k (copy_bytes a1 a2 l m1 m2)
+      = If within_bool a2 l k
+        Then M.find (plusPtr a1 (k - a2)) m1
+        Else M.find k m2.
 Proof.
   intros.
   unfold copy_bytes, drop_range, keep_keys.
@@ -204,12 +211,12 @@ Proof.
     - rewrite <- H; assumption.
     - rewrite !F.empty_o; trivial.
     - destruct (within_bool a1 l k0) eqn:Heqe2; simpl.
-        destruct (N.eq_dec (k0 - a1 + a2) k); subst.
-          replace (k0 - a1 + a2 - a2 + a1) with k0 by nomega.
+        destruct (N.eq_dec (plusPtr a2 (k0 - a1)) k); subst.
+          replace (plusPtr a1 (plusPtr a2 (k0 - a1) - a2)) with k0 by nomega.
           rewrite !F.add_eq_o; trivial.
-        assert (k0 <> k - a2 + a1) by nomega.
+        assert (k0 <> plusPtr a1 (k - a2)) by nomega.
         rewrite !F.add_neq_o; trivial.
-      assert (k0 <> k - a2 + a1) by nomega.
+      assert (k0 <> plusPtr a1 (k - a2)) by nomega.
       rewrite F.add_neq_o; trivial.
     - unfold not; intros.
       destruct (proj1 (in_mapsto_iff _ _ _) H); clear H.
@@ -240,7 +247,7 @@ Proof.
   }
 Qed.
 
-Lemma copy_bytes_zero {elt} addr1 addr2 (m1 m2 : M.t elt) :
+Lemma copy_bytes_zero {elt A} (addr1 addr2 : Ptr A) (m1 m2 : M.t elt) :
   M.Equal (elt:=elt) (copy_bytes addr1 addr2 0 m1 m2) m2.
 Proof.
   apply F.Equal_mapsto_iff; split; intros;
@@ -250,30 +257,30 @@ Proof.
   nomega.
 Qed.
 
-Lemma copy_bytes_idem d len elt (m : M.t elt) :
+Lemma copy_bytes_idem {A} (d : Ptr A) len elt (m : M.t elt) :
   M.Equal (copy_bytes d d len m m) m.
 Proof.
   apply F.Equal_mapsto_iff; split; intros;
   [ apply copy_bytes_mapsto in H
   | apply copy_bytes_mapsto ];
   destruct (within_bool d len k) eqn:Heqe; simpl in *; trivial;
-  revert H; replace (k - d + d) with k by nomega; trivial.
+  revert H; replace (plusPtr d (k - d)) with k by nomega; trivial.
 Qed.
 
-Lemma copy_bytes_find_at : forall b k l elt (m1 m2 : M.t elt),
+Lemma copy_bytes_find_at : forall A (b k : Ptr A) l elt (m1 m2 : M.t elt),
   0 < l -> M.find k (copy_bytes b k l m1 m2) = M.find b m1.
 Proof.
   intros.
   rewrite copy_bytes_find.
   assert (within_bool k l k = true) by nomega.
   rewrite H0; simpl.
-  replace (k - k + b) with b by nomega.
+  replace (plusPtr b (k - k)) with b by nomega.
   reflexivity.
 Qed.
 
-Lemma increase_heap_ceiling : forall n m r,
-  P.for_all (fun addr sz => addr + sz <=? n) r ->
-  P.for_all (fun addr sz => addr + sz <=? n + m) r.
+Lemma increase_heap_ceiling : forall A (n : Ptr A) m r,
+  P.for_all (fun (addr : Ptr A) sz => plusPtr addr sz <=? n) r ->
+  P.for_all (fun (addr : Ptr A) sz => plusPtr addr sz <=? plusPtr n m) r.
 Proof.
   intros.
   eapply for_all_impl; auto;
