src/Memory.v
@@ -1,8 +1,120 @@
 Require Import
+  ByteString.Lib.Nomega
   Coq.NArith.NArith
-  Coq.Strings.Ascii.
+  Coq.Strings.Ascii
+  Coq.Structures.DecidableTypeEx
+  Coq.Structures.OrderedType
+  Coq.Structures.OrderedTypeEx.
+
+Generalizable All Variables.
 
 Definition Ptr (A : Type) := N.
 Definition Size := N.
 Definition Word := Ascii.ascii.
 Definition Zero := Ascii.zero.
+
+Definition plusPtr `(ptr : Ptr A) (n : Size) := (ptr + n)%N.
+Definition minusPtr `(ptr : Ptr A) (n : Size) := (ptr - n)%N.
+
+Module Ptr_as_OT <: UsualOrderedType.
+  Definition t:=Ptr Word.
+  Definition eq:=@eq (Ptr Word).
+  Definition eq_refl := @eq_refl t.
+  Definition eq_sym := @eq_sym t.
+  Definition eq_trans := @eq_trans t.
+
+  Definition lt := N.lt.
+  Definition lt_trans := N.lt_trans.
+  Definition lt_not_eq := N.lt_neq.
+
+  Definition compare x y : Compare lt eq x y.
+  Proof.
+  case_eq (x ?= y)%N; intro.
+  - apply EQ. now apply N.compare_eq.
+  - apply LT. assumption.
+  - apply GT. now apply N.gt_lt.
+  Defined.
+
+  Definition eq_dec := N.eq_dec.
+End Ptr_as_OT.
+
+Module Ptr_as_DT <: UsualDecidableType := Ptr_as_OT.
+
+Local Open Scope N_scope.
+
+Corollary succ_sub_one : forall n,
+  N.succ n - 1 = n.
+Proof. nomega. Qed.
+
+Corollary succ_one_sub : forall n,
+  N.succ n - n = 1.
+Proof. intros; rewrite N.sub_succ_l; nomega. Qed.
+
+Corollary plusPtr_zero : forall A (addr : Ptr A),
+  plusPtr addr 0 = addr.
+Proof. intros; nomega. Qed.
+
+Corollary plusPtr_add : forall A (addr : Ptr A) n m,
+  plusPtr (A:=A) (plusPtr addr n) m = plusPtr addr (n + m).
+Proof. intros; nomega. Qed.
+
+Corollary plusPtr_succ : forall A (addr : Ptr A) n,
+  plusPtr (A:=A) (plusPtr addr n) 1 = plusPtr addr (N.succ n).
+Proof. intros; nomega. Qed.
+
+Corollary plusPtr_sub : forall A (addr : Ptr A) n m,
+  m <= n -> minusPtr (A:=A) (plusPtr addr n) m = plusPtr addr (n - m).
+Proof. intros; symmetry; apply N.add_sub_assoc; nomega. Qed.
+
+Corollary plusPtr_sub_r : forall A (addr : Ptr A) n m,
+  n <= addr -> n <= m
+    -> plusPtr (A:=A) (minusPtr addr n) m = plusPtr addr (m - n).
+Proof. intros; nomega. Qed.
+
+Corollary plusPtr_comm : forall A (addr : Ptr A) n m,
+  plusPtr (A:=A) (plusPtr addr n) m = plusPtr (A:=A) (plusPtr addr m) n.
+Proof. intros; nomega. Qed.
+
+Corollary minusPtr_add : forall A (addr : Ptr A) n m,
+  minusPtr (A:=A) (minusPtr addr n) m = minusPtr addr (n + m).
+Proof. intros; nomega. Qed.
+
+Corollary minusPtr_zero : forall A (addr : Ptr A),
+  minusPtr addr 0 = addr.
+Proof. intros; nomega. Qed.
+
+Corollary minusPtr_succ : forall A (addr : Ptr A) n,
+  n <= addr -> minusPtr (A:=A) (minusPtr addr 1) n = minusPtr addr (N.succ n).
+Proof. intros; nomega. Qed.
+
+Corollary minusPtr_sub : forall A (addr : Ptr A) n m,
+  m <= n -> minusPtr (A:=A) (plusPtr addr m) n = minusPtr addr (n - m).
+Proof. intros; nomega. Qed.
+
+Hint Rewrite N.add_0_r : ptr.
+Hint Rewrite N.add_sub : ptr.
+Hint Rewrite N.add_succ_l : ptr.
+Hint Rewrite N.sub_diag : ptr.
+Hint Rewrite N.sub_succ : ptr.
+Hint Rewrite N.peano_rec_succ : ptr.
+Hint Rewrite succ_sub_one : ptr.
+Hint Rewrite succ_one_sub : ptr.
+Hint Rewrite plusPtr_zero : ptr.
+Hint Rewrite plusPtr_add : ptr.
+Hint Rewrite plusPtr_sub : ptr.
+Hint Rewrite plusPtr_succ : ptr.
+Hint Rewrite minusPtr_zero : ptr.
+Hint Rewrite minusPtr_add : ptr.
+Hint Rewrite minusPtr_sub : ptr.
+Hint Rewrite minusPtr_succ : ptr.
+
+Ltac rewrite_ptr :=
+  repeat (
+    autorewrite with ptr; try nomega;
+    repeat match goal with
+    | [ |- context[N.succ _ - _] ] =>
+      rewrite N.sub_succ_l; [|nomega]
+    | [ |- context[N.peano_rec _ _ _ (_ + 1)] ] =>
+      rewrite N.add_1_r
+    end);
+  first [ auto | discriminate | congruence | nomega | idtac ].
